Adapt handlers to higher-order, #59 #68

Coq/src/HigherOrder/Handler.v
@@ -21,67 +21,48 @@ Fixpoint runChoice A (fc : Free C__Choice A) : Tree A :=
   | impure (ext (schoice mid) pf _) => Branch mid (runChoice (pf true)) (runChoice (pf false))
   end.
 
-Fixpoint runState A (n : nat * nat) (fc : Prog A) : Prog__SC A.
-  destruct fc.
-  - give_up.
-  - destruct e.
-    destruct s.
-    + give_up.
-    + destruct s.
-      * destruct s.
-        apply impure.
-        apply ext with (s := inl (ssharing n A)).
-        -- intros.
-           apply runState.
-           ++ apply n.
-           ++ apply f.
-              apply pcont.
-              simpl. simpl in *.
-              Admitted.
+Fixpoint runState A (n : nat * nat) (fc : Prog A) : Prog__SC A :=
+  match fc with
+  | pure x => pure x
+  | impure (ext (inl (sget _))    pf _) => runState n  (pf (pget n))
+  | impure (ext (inl (sput s'))   pf _) => runState s' (pf (pput s'))
+  | impure (ext (inr (inr sfail)) _ _)  => Fail__SC
+  | impure (ext (inr (inr (schoice mid))) pf _) => Choice__SC mid (runState n (pf true)) (runState n (pf false))
+  | impure (ext (inr (inl (ssharing m T) as s))  pf pfx) =>
+    let s : @Shape _ NDShare__SC := inl (ssharing m T)
+    in impure (ext s (fun p : @Pos _ NDShare__SC s => runState n (pf p))
+                   (fun p : @PosX _ NDShare__SC s => runState n (pfx p)))
+  end.
 
-  (* match fc with *)
-  (* | pure x => pure x *)
-  (* | impure (ext (inl (sget _))    pf _) => runState n  (pf (pget n)) *)
-  (* | impure (ext (inl (sput s'))   pf _) => runState s' (pf (pput s')) *)
-  (* | impure (ext (inr (inr sfail)) _ _)  => Fail__SC *)
-  (* | impure (ext (inr (inr (schoice mid))) pf _) => Choice__SC mid (runState n (pf true)) (runState n (pf false)) *)
-  (* | impure (ext (inr (inl (ssharing m _ as s)))  pf pfx) => *)
-  (*   let s : @Shape _ NDShare__SC := (inl (ssharing n A)) *)
-  (*   in impure (ext s (fun p : @Pos _ NDShare__SC s => runState n (pf p)) *)
-  (*                  (fun p : @PosX _ NDShare__SC s => match p with pshared _ => fs end)) *)
-  (*   (* Share'__SC m (runState n (pfx (pshared s))) (fun x => (pf (pcont s x))) *) *)
-  (* end. *)
+Definition tripl A B C (p : A * B) (c : C) : A * B * C :=
+  let '(a,b) := p in (a,b,c).
 
-(* Definition tripl A B C (p : A * B) (c : C) : A * B * C := *)
-(*   let '(a,b) := p in (a,b,c). *)
+Fixpoint nameChoices  A (next : nat) (scope : nat * nat) (fs : Prog__SC A)
+  : Free C__Choice A :=
+   match fs with
+  | pure x => pure x
+  | impure (ext (inl (ssharing m X)) pf pfx) =>
+    let s : @Shape _ C__Sharing := ssharing m X
+    in nameChoices 1 m (pfx (pshared s)) >>=
+                   fun x => nameChoices next scope (pf (pcont s x))
+  | impure (ext (inr sfail)        pf _) => Fail__C
+  | impure (ext (inr (schoice _))  pf _) =>
+    let l := nameChoices (next + 1) scope (pf true) in
+    let r := nameChoices (next + 1) scope (pf false)
+    in Choice__C (Some (tripl scope next)) l r
+  end.
+    
+Fixpoint runSharing A (fs : Free (C__Comb C__Sharing C__Choice) A) : Free C__Choice A :=
+  match fs with
+  | pure x => pure x
+  | impure (ext (inl (ssharing n X))  pf pfx) =>
+    let s : @Shape _ C__Sharing := ssharing n X
+    in nameChoices 1 n (pfx (pshared s)) >>=
+                   fun x => runSharing (pf (pcont s x))
+  | impure (ext (inr sfail)         _ _)  => Fail__C
+  | impure (ext (inr (schoice mid)) pf _) =>
+    Choice__C mid (runSharing (pf true)) (runSharing (pf false))
+  end.
 
-(* Fixpoint runSharing A (fs : Free (C__Comb C__Sharing C__Choice) A) : Free C__Choice A := *)
-(*   let fix nameChoices (next : nat) (scope : nat * nat) (scopes : list (nat * nat)) (fs : Prog__SC A) *)
-(*   : Free C__Choice A  := *)
-(*       match fs with *)
-(*       | pure x => pure x *)
-(*       | impure (ext (inl (sbsharing n)) pf) => *)
-(*         nameChoices 1 n (cons n scopes) (pf (pbsharing n)) *)
-(*       | impure (ext (inl (sesharing n)) pf) => *)
-(*         match scopes with *)
-(*         | cons _ (cons j js) as ks => nameChoices next j ks (pf (pesharing n))  *)
-(*         | _                        => runSharing (pf (pesharing n)) *)
-(*         end *)
-(*       | impure (ext (inr sfail)        pf) => Fail__C *)
-(*       | impure (ext (inr (schoice _))  pf) => *)
-(*         let l := nameChoices (next + 1) scope scopes (pf true) in *)
-(*         let r := nameChoices (next + 1) scope scopes (pf false) *)
-(*         in Choice__C (Some (tripl scope next)) l r *)
-(*       end *)
-(*   in match fs with *)
-(*      | pure x => pure x *)
-(*      | impure (ext (inl (sbsharing n))  pf) => *)
-(*        nameChoices 1 n (cons n nil) (pf (pbsharing n)) *)
-(*      | impure (ext (inl (sesharing n))  pf) => runSharing (pf (pesharing n)) *)
-(*      | impure (ext (inr sfail)         _)  => Fail__C *)
-(*      | impure (ext (inr (schoice mid)) pf) => *)
-(*        Choice__C mid (runSharing (pf true)) (runSharing (pf false)) *)
-(*      end. *)
-
-(* Definition handle A `{Normalform A A} (fs : Prog A) : list A := *)
-(*   collectVals (runChoice (runSharing (runState (0,0) (nf fs)))). *)
+Definition handle A `{Normalform A A} (fs : Prog A) : list A :=
+  collectVals (runChoice (runSharing (runState (0,0) (nf fs)))).
