Coq/src/HigherOrder/Example.v
@@ -1,0 +1,349 @@
+Require Import Thesis.HigherOrder.Base.
+Require Import Thesis.HigherOrder.DataM.
+Require Import Thesis.HigherOrder.Effect.
+Require Import Thesis.HigherOrder.Handler.
+Require Import Thesis.HigherOrder.Prog.
+
+Require Import Lists.List.
+
+Import List.ListNotations.
+
+Set Implicit Arguments.
+
+Definition coin := Coin__Bool.
+Definition share := Share.
+Definition const := fun A (x _ : A) => x.
+
+Section exB.
+  Example example1 : Prog bool := coin.
+  Example res_example1 := [true; false].
+
+  Example example2 : Prog bool := coin ? coin.
+  Example res_example2 := [true; false; true; false].
+  
+  Example example3 : Prog bool :=  share coin >>= fun fx => fx ? fx.
+  Example res_example3 := [true; false; true; false].
+  
+  Example exOr0 : Prog bool := orM coin (pure false).
+  Example res_exOr0 := [true; false].
+  
+  Example exOr1 : Prog bool := orM coin coin.
+  Example res_exOr1 := [true; true; false].
+  
+  Example exOr2 : Prog bool := share coin >>= fun fx => orM fx fx.
+  Example res_exOr2 := [true; false].
+  
+  Example exOr2a : Prog bool :=
+    share coin >>= fun fx => orM (pure false) (orM fx fx).
+  Example res_exOr2a := [true; false].
+  
+  Example exOr2b : Prog bool :=
+    share coin >>= fun fx => orM (pure true) (orM fx fx).
+  Example res_exOr2b := [true].
+  
+  Example exOr3 : Prog bool := orM (coin ? coin) (pure true).
+  Example res_exOr3 := [true; true; true; true].
+  
+  Example exOr3a : Prog bool := orM (coin ? coin) coin.
+  Example res_exOr3a := [true; true; false; true; true; false].
+  
+  Example exOr3b : Prog bool := orM coin (coin ? coin).
+  Example res_exOr3b := [true; true; false; true; false].
+  
+  Example exOr3c : Prog bool := orM (coin ? coin) (coin ? coin).
+  Example res_exOr3c := [true; true; false; true; false; true; true; false; true; false].
+  
+  (* here we share, even though nothing is shared *)
+  Example exOr4 : Prog bool := share coin >>= fun fx => orM fx coin.
+  Example res_exOr4 := [true; true; false].
+  
+  Example exOrShare : Prog bool := share coin >>= fun fx => orM coin fx.
+  Example res_exOrShare := [true; true; false].
+  
+  Example exOr6 : Prog bool := share coin >>= fun fx => orM fx (orM fx coin).
+  Example res_exOr6 := [true; true; false].
+  
+  Example exOr7 : Prog bool := share coin >>= fun fx => orM coin (orM fx fx).
+  Example res_exOr7 := [true; true; false].
+  
+  Example exOr7a : Prog bool := share coin >>= fun fx => orM (pure true) (orM fx fx).
+  Example res_exOr7a := [true].
+  
+  Example exOr7b : Prog bool := share coin >>= fun fx => orM (pure false) (orM fx fx).
+  Example res_exOr7b := [true; false].
+  
+  Example exShareConst : Prog bool := share coin >>= fun fx => const fx fx.
+  Example res_exShareConst := [true; false].
+  
+  Example exShareConstOrR : Prog bool := share coin >>= fun fx => orM fx (const fx fx).
+  Example res_exShareConstOrR := [true; false].
+  
+  Example exShareConstOrL : Prog bool := share coin >>= fun fx => orM (const fx fx) fx.
+  Example res_exShareConstOrL := [true; false].
+  
+  Example exShareConstOrR2 : Prog bool := share coin >>= fun fx => orM (pure true) (const fx fx).
+  Example res_exShareConstOrR2 := [true].
+  
+  Example exFailed : Prog bool := share Fail >>= fun fx => const (pure true) fx.
+  Example res_exFailed := [true].
+  
+  Example exHead : Prog bool := headM (consM coin Fail).
+  Example res_exHead := [true; false].
+  
+  Example exOrShareShare : Prog bool :=
+    share coin >>=
+          fun fx =>
+            share coin >>=
+                  fun fy =>
+                    orM fx (orM fy (orM fx fy)).
+  Example res_exOrShareShare := [true; true; false].
+  
+  Example exOrShareNested : Prog bool :=
+    share coin >>= fun fx =>
+                     orM fx (share coin >>= fun fy =>
+                                              orM fy (orM fx fy)).
+  Example res_exOrShareNested := [true; true; false].
+  
+  Example exShareNestedChoiceOr : Prog bool :=
+    share ((pure true ? pure false) ? (pure true ? pure false)) >>=
+          fun fx => orM fx fx.
+  Example res_exShareNestedChoiceOr := [true; false; true; false].
+  
+  Example exShareIgnoreShare : Prog bool :=
+    share coin >>= fun fx => const (pure true) (share fx >>= fun fy => orM fy fy).
+  Example res_exShareIgnoreShare := [true].
+  
+  Example exRepeatedShare : Prog bool :=
+    share coin >>= fun fx => share fx >>= fun fy => orM fy fy.
+  Example res_exRepeatedShare := [true; false].
+  
+  Definition exBs := [(example1, res_example1);
+                        (example2, res_example2);
+                        (example3, res_example3);
+                        (exOr0, res_exOr0);
+                        (exOr1, res_exOr1);
+                        (exOr2, res_exOr2);
+                        (exOr2a, res_exOr2a);
+                        (exOr2b, res_exOr2b);
+                        (exOr3, res_exOr3);
+                        (exOr3a, res_exOr3a);
+                        (exOr3b, res_exOr3b);
+                        (exOr3c, res_exOr3c);
+                        (exOr4, res_exOr4);
+                        (exOrShare, res_exOrShare);
+                        (exOr6, res_exOr6);
+                        (exOr7, res_exOr7);
+                        (exOr7a, res_exOr7a);
+                        (exOr7b, res_exOr7b);
+                        (exShareConst, res_exShareConst);
+                        (exShareConstOrR, res_exShareConstOrR);
+                        (exShareConstOrL, res_exShareConstOrL);
+                        (exShareConstOrR2, res_exShareConstOrR2);
+                        (exFailed, res_exFailed);
+                        (exHead, res_exHead);
+                        (exOrShareShare, res_exOrShareShare);
+                        (exOrShareNested, res_exOrShareNested);
+                        (exShareNestedChoiceOr, res_exShareNestedChoiceOr);
+                        (exShareIgnoreShare, res_exShareIgnoreShare);
+                        (exRepeatedShare, res_exRepeatedShare)].
+  
+  Lemma tests__exBs : Forall (fun '(p,r) => handle p = r) exBs.
+  Proof. repeat econstructor. Qed.
+End exB.
+
+Section exPB.
+  Example exDup : Prog (Pair bool bool) := dup coin.
+  Example res_exDup := [Pair' (pure true) (pure true)
+                        ; Pair' (pure true) (pure false)
+                        ; Pair' (pure false) (pure true)
+                        ; Pair' (pure false) (pure false)].
+  
+  Example exDupShare : Prog (Pair bool bool) := share coin >>= fun x => dup x.
+  Example res_exDupShare := [Pair' (pure true) (pure true)
+                             ; Pair' (pure false) (pure false)].
+  
+  Example exDupShare2 : Prog (Pair bool bool) := dupShare coin.
+
+  Example res_exDupShare2 := [Pair' (pure true) (pure true)
+                              ; Pair' (pure false) (pure false)].
+  
+  Example exDupFailed : Prog (Pair bool bool) := share Fail >>= fun x => dup (const (pure true) x).
+  Example res_exDupFailed := [Pair' (pure true) (pure true)].
+  
+  Example exDupFirst : Prog (Pair bool bool) := dup (firstM (pairM coin (@Fail bool))).
+  Example res_exDupFirst := [Pair' (pure true) (pure true)
+                             ; Pair' (pure true) (pure false)
+                             ; Pair' (pure false) (pure true)
+                             ; Pair' (pure false) (pure false)].
+  
+  Example exDupShareFirst : Prog (Pair bool bool) := dupShare (@firstM bool bool (pairM coin Fail)).
+  Example res_exDupShareFirst :=  [Pair' (pure true) (pure true); Pair' (pure false) (pure false)].
+
+  
+  Example exShareNestedChoice : Prog (Pair bool bool) :=
+    share ((pure true ? pure false) ? (pure true ? pure false)) >>=
+          fun fx => pairM fx fx.
+  Example res_exShareNestedChoice := [Pair' (pure true) (pure true) 
+                                      ; Pair' (pure false) (pure false)
+                                      ; Pair' (pure true) (pure true)
+                                      ; Pair' (pure false) (pure false)].
+  
+  Definition exPBs := [(exDup, res_exDup)
+                       ; (exDupShare, res_exDupShare)
+                       ; (exDupShare2, res_exDupShare2)
+                       ; (exDupFailed, res_exDupFailed)
+                       ; (exDupFirst, res_exDupFirst)
+                       ; (exDupShareFirst, res_exDupShareFirst)
+                       ; (exShareNestedChoice, res_exShareNestedChoice)].
+
+  Lemma tests__exPBs : Forall (fun '(p,r) => handle p = r) exPBs.
+  Proof. repeat econstructor. Qed.
+End exPB.
+
+Section exLB.
+  Arguments nilM {_}.
+  Arguments Nil' {_}.
+
+  Example exDupl : Prog (List bool) := dupl (headM (consM coin Fail)).
+  Example res_exDupl := [Cons' (pure true) (consM (pure true) nilM)
+                         ; Cons' (pure true) (consM (pure false) nilM)
+                         ; Cons' (pure false) (consM (pure true) nilM)
+                         ; Cons' (pure false) (consM (pure false) nilM)].
+
+  Example exDupl2 : Prog (List bool) := consM (headM (consM coin Fail))
+                                           (consM (headM (consM coin Fail)) nilM).
+  Example res_exDupl2 := [Cons' (pure true) (consM (pure true) nilM)
+                          ; Cons' (pure true) (consM (pure false) nilM)
+                          ; Cons' (pure false) (consM (pure true) nilM)
+                          ; Cons' (pure false) (consM (pure false) nilM)].
+
+  Example exDuplShare : Prog (List bool) := duplShare (headM (consM coin Fail)).
+  Example res_exDuplShare := [Cons' (pure true) (consM (pure true) nilM)
+                              ; Cons' (pure false) (consM (pure false) nilM)].
+
+  Example exShareNestedChoice2 : Prog (List bool) :=
+    share (pure true ? (pure false ? pure true)) >>=
+          fun fx => share coin >>= fun fy => consM fx (consM fy (consM fx (consM fy nilM))).
+
+  Example res_exShareNestedChoice2 :=
+    [Cons' (pure true) (consM (pure true) (consM (pure true) (consM (pure true) nilM)))
+     ; Cons' (pure true) (consM (pure false) (consM (pure true) (consM (pure false) nilM)))
+     ; Cons' (pure false) (consM (pure true) (consM (pure false) (consM (pure true) nilM)))
+     ; Cons' (pure false) (consM (pure false) (consM (pure false) (consM (pure false) nilM)))
+     ; Cons' (pure true) (consM (pure true) (consM (pure true) (consM (pure true) nilM)))
+     ; Cons' (pure true) (consM (pure false) (consM (pure true) (consM (pure false) nilM)))].
+
+  Example exOrShareNestedList : Prog (List bool) :=
+    share coin >>= fun fx =>
+                     consM fx (share coin >>= fun fy =>
+                                                consM fy (consM fx (consM fy nilM))).
+  Example res_exOrShareNestedList :=
+    [Cons' (pure true) (consM (pure true) (consM (pure true) (consM (pure true) nilM)))
+     ; Cons' (pure true) (consM (pure false) (consM (pure true) (consM (pure false) nilM)))
+     ; Cons' (pure false) (consM (pure true) (consM (pure false) (consM (pure true) nilM)))
+     ; Cons' (pure false) (consM (pure false) (consM (pure false) (consM (pure false) nilM)))].
+
+  Definition exLBs := [(exDupl, res_exDupl)
+                       ; (exDupl2,  res_exDupl2)
+                       ; (exDuplShare, res_exDuplShare)
+                       ; (exShareNestedChoice2, res_exShareNestedChoice2)
+                       ; (exOrShareNestedList, res_exOrShareNestedList)].
+
+  Lemma tests__exLBs : Forall (fun '(p,r) => handle p = r) exLBs.
+  Proof. repeat econstructor. Qed.
+
+End exLB.
+              
+Section exLPB.
+
+ Example exShareSingleton : Prog (Pair (List bool) (List bool)) :=
+   Share (consM (pure true ? pure false) nilM) >>= fun fx => pairM fx fx.
+ Example res_exShareSingleton := [Pair' (pure (Cons' (pure true) nilM))
+                                        (pure (Cons' (pure true) nilM))
+                                  ; Pair' (pure (Cons' (pure false) nilM))
+                                          (pure (Cons' (pure false) nilM))].
+
+   Fixpoint recList' (n : nat) (xs : List bool) : Prog (List bool) :=
+     match n with
+     | 0 => Fail
+     | S n => match xs with
+             | Nil' _ => nilM
+             | Cons' fy fys =>
+               Share fys >>= fun fys' => consM (notM fy) (fys' ? fys' >>= fun zs => recList' n zs)
+             end
+     end.
+
+   
+   Definition recList (fxs : Prog (List bool)) : Prog (List bool) :=
+     fxs >>= fun xfps => lengthM xfps >>= fun fuel => recList' (fuel + 1) xfps.
+
+   Example exRecList : Prog (Pair (List bool) (List bool)) :=
+     Share (recList (consM (pure true) (consM (pure false) nilM))) >>= fun fx => pairM fx fx.
+   Example res_exRecList :=  [ Pair' (consM (pure false) (consM (pure false) nilM))
+                                     (consM (pure false) (consM (pure false) nilM))
+                             ; Pair' (consM (pure false) (consM (pure true) nilM))
+                                     (consM (pure false) (consM (pure true) nilM))
+                             ; Pair' (consM (pure false) (consM (pure true) nilM))
+                                     (consM (pure false) (consM (pure true) nilM))].
+   
+   Definition exLPBs := [(exShareSingleton, res_exShareSingleton)
+                         ; (exRecList, res_exRecList)].
+   
+  Lemma tests__exLPBs : Forall (fun '(p,r) => handle p = r) exLPBs.
+  Proof. repeat econstructor. Qed.
+End exLPB.
+
+Section Extra.
+  Example exSkipIds : Prog bool :=
+    Share coin >>= fun fx => const coin (const fx fx).
+  Example res_exSkipIds := [true; false].
+
+  Lemma lem_exSkipIDs : handle exSkipIds = res_exSkipIds.
+  Proof. reflexivity. Qed.
+
+  Example exShareInShare : Prog (Pair bool bool) :=
+    Share (Share coin >>= fun fx => orM fx fx) >>= fun fy => pairM fy fy.
+  Example res_exShareInShare := [Pair' (pure true) (pure true)
+                                 ; Pair' (pure false) (pure false)].
+  Lemma lem_exShareInShare : handle exShareInShare = res_exShareInShare.
+  Proof. reflexivity. Qed.
+
+  Example exShareListInShare : Prog (Pair (List bool) (List bool)) :=
+    Share (Share (consM coin (consM coin nilM)) >>=
+                 fun fx => appM fx fx) >>= fun fy => pairM fy fy.
+  
+  Example res_exShareListInShare :=
+    [Pair' (consM (pure true) (consM (pure true) (consM (pure true) (consM (pure true) nilM))))
+           (consM (pure true) (consM (pure true) (consM (pure true) (consM (pure true) nilM))))
+     ; Pair' (consM (pure true) (consM (pure false) (consM (pure true) (consM (pure false) nilM))))
+             (consM (pure true) (consM (pure false) (consM (pure true) (consM (pure false) nilM))))
+     ; Pair' (consM (pure false) (consM (pure true) (consM (pure false) (consM (pure true) nilM))))
+             (consM (pure false) (consM (pure true) (consM (pure false) (consM (pure true) nilM))))
+     ; Pair' (consM (pure false) (consM (pure false) (consM (pure false) (consM (pure false) nilM))))
+             (consM (pure false) (consM (pure false) (consM (pure false) (consM (pure false) nilM))))].
+  Lemma lem_exShareListInShare : handle exShareListInShare = res_exShareListInShare.
+  Proof. reflexivity. Qed.
+
+  Example exSharePutPos : Prog (List bool) :=
+    Share (Share (consM coin nilM) >>= fun fx => appM fx fx) >>= fun fy => appM fy fy.
+  
+  Example res_exSharePutPos := [Cons' (pure true) (consM (pure true) (consM (pure true) (consM (pure true) nilM)))
+                                ; Cons'  (pure false) (consM (pure false) (consM (pure false) (consM (pure false) nilM)))].
+  Lemma lem_exSharePutPos : handle exSharePutPos = res_exSharePutPos.
+  Proof. reflexivity. Qed.
+
+  Example exShareListInRepeatedShare : Prog (List bool) :=
+    Share (Share (consM coin nilM) >>= fun fx => appM fx fx) >>=
+          fun fy => Share coin >>= fun fz => Share coin >>= fun fa => consM fz (consM fa fy).
+  Example res_exShareListInRepeatedShare :=
+    [Cons' (pure true) (consM (pure true) (consM (pure true) (consM (pure true) nilM)))
+     ; Cons' (pure true) (consM (pure true) (consM (pure false) (consM (pure false) nilM)))
+     ;  Cons' (pure true) (consM (pure false) (consM (pure true) (consM (pure true) nilM)))
+     ;  Cons' (pure true) (consM (pure false) (consM (pure false) (consM (pure false) nilM)))
+     ;  Cons' (pure false) (consM (pure true) (consM (pure true) (consM (pure true) nilM)))
+     ;  Cons' (pure false) (consM (pure true) (consM (pure false) (consM (pure false) nilM)))
+     ;  Cons' (pure false) (consM (pure false) (consM (pure true) (consM (pure true) nilM)))
+     ;  Cons' (pure false) (consM (pure false) (consM (pure false) (consM (pure false) nilM)))].
+  Lemma lem_exShareListInRepeatedShare : handle exShareListInRepeatedShare = res_exShareListInRepeatedShare.
+  Proof. reflexivity. Qed.
+End Extra.
